Implented path induction tactic, started rewriting proofs using that.

Tltt/Tactics.lean
@@ -3,7 +3,6 @@ import Lean.Elab.Tactic.Location
 import Lean.Elab.Tactic.Rewrite
 
 import Tltt.ObjLang
-import Tltt.Hott
 
 open Lean.Parser.Tactic (rwRuleSeq location)
 open Lean.Elab.Term (withSynthesize)
@@ -12,6 +11,8 @@ open Lean.Elab.Tactic (
   TacticM
   elabTerm
   expandOptLocation
+  getFVarId
+  getGoals
   getMainGoal
   getMainTarget
   replaceMainGoal
@@ -19,11 +20,14 @@ open Lean.Elab.Tactic (
   withMainContext
   withRWRulesSeq
 )
+open Lean.Elab (throwUnsupportedSyntax)
 open Lean.Meta (
   AssertAfterResult
   MetaM
   RewriteResult
+  forallBoundedTelescope
   forallMetaTelescopeReducing
+  forallTelescopeReducing
   getLevel
   getMVarsNoDelayed
   inferType
@@ -31,28 +35,35 @@ open Lean.Meta (
   isTypeCorrect
   kabstract
   matchHelper?
-  mkFreshLevelMVar
+  mkAppM
+  mkForallFVars
   mkFreshExprMVar
+  mkFreshExprSyntheticOpaqueMVar
+  mkFreshLevelMVar
+  mkLambdaFVars
   postprocessAppMVars
   throwTacticEx
   whnfD
+  whnfI
+  withLocalDecl
 )
 open Lean (
   BinderInfo
   Expr
   FVarId
   Level
+  LocalDecl
   MVarId
+  Name
   Occurrences
   Syntax
   indentExpr
   instantiateMVars
-  mkApp
   mkApp2
   mkApp3
   mkApp4
   mkAppN
-  mkConst
+  mkFreshFVarId
   mkFreshMVarId
 )
 
@@ -62,44 +73,46 @@ set_option autoImplicit false
 
 namespace Hott.Tactic
 
-/-- If given `lift.{u} α`, returns `(u, α)` -/
+/-- If given `lift.{u} α`, returns `(u, α)`. -/
 def _root_.Lean.Expr.lift? (e : Expr) : MetaM (Option (Level × Expr)) := do
-  let type ← Lean.Meta.mkFreshExprMVar (← Lean.Meta.mkConstWithFreshMVarLevels ``Hott.liftedU)
-  let u ← Lean.Meta.mkFreshLevelMVar
+  let u ← mkFreshLevelMVar
+  let type ← mkFreshExprMVar (Expr.const ``Hott.liftedU [u])
   let lifted := Expr.app (.const ``Hott.lift [u]) type
   if ← isDefEq e lifted then
     return some (u, type)
   else
     return none
 
+def _root_.Lean.Expr.lift! (e : Expr) : MetaM (Level × Expr) := do
+  let some (u, t) ← e.lift? | throwError "{indentExpr e} is not an object-level type"
+  return (u, t)
 
-/--
-Lift `α` into `^α`.
--/
+/-- Lifts `α` into `^α`. -/
 @[inline]
 def _root_.Lean.Expr.liftWith (e : Expr) (u : Level) : Expr :=
   .app (.const ``Hott.lift [u]) e
 
-/--
-If `e` is a lifted type `^α`, returns `α`.
--/
+/-- If `e` is a lifted type `^α`, returns `α`. -/
 @[inline]
 def _root_.Lean.Expr.objType? (e : Expr) : Option Expr :=
   e.app1? ``Hott.lift
 
+/-- Given `^α`, returns `α`. -/
 @[inline]
-def _root_.Lean.Expr.objType (e : Expr) : MetaM Expr := do
-  let some t := e.objType? | throwError "{indentExpr e} is not an object-level type"
+def _root_.Lean.Expr.objType! (e : Expr) : MetaM Expr := do
+  let some (_, t) ← e.lift? | throwError "{indentExpr e} is not an object-level type"
   return t
 
-    
+
+/-- Given `x : lift.{u} α`, returns (u, α). -/
 @[inline]
 def inferObjType (e : Expr) : MetaM (Level × Expr) := do
   let t ← inferType e
-  match ← t.lift? with
-  | some x => return x
-  | none => throwError "expression{indentExpr e}\nhas type{indentExpr t}\nwhich is not an object-level type"
+  let some result ← t.lift?
+    | throwError "expression{indentExpr e}\nhas type{indentExpr t}\nwhich is not an object-level type"
+  return result
 
+/-- Given `Id.{u} {α} x y`, returns `(u, α, x, y)`. -/
 @[inline]
 def _root_.Lean.Expr.id? (e : Expr) : MetaM (Option (Level × Expr × Expr × Expr)) := do
   let u ← mkFreshLevelMVar
@@ -112,6 +125,7 @@ def _root_.Lean.Expr.id? (e : Expr) : MetaM (Option (Level × Expr × Expr × Ex
   else
     return none
 
+/-- Given `x : ^α` where `α : ^U.{u}`, returns `u` -/
 def getObjLevel (e : Expr) : MetaM Level := do
   let t ← inferType e
   let u ← mkFreshLevelMVar
@@ -122,58 +136,38 @@ def getObjLevel (e : Expr) : MetaM Level := do
     throwError "expression{indentExpr e}\nhas type{indentExpr t}\nwhich is not an object-level type"
     
 
-/--
-Lift `α` into `^α`.
--/
+/-- Lift `α` into `^α`. -/
 @[inline]
 def _root_.Lean.Expr.lift (e : Expr) : MetaM Expr := do
   let u ← getObjLevel e
-  return .app (.const ``Hott.lift [u]) e
-
-universe u in
-example : lift.{u+1} U.{u} = liftedU.{u} := by rfl
-
----  Object-level rewrite: rewriteₒ
-def replaceLocalDeclObjCore (mvarId : MVarId) (fvarId : FVarId) (typeNew : Expr)
-                            (eqProof : Expr) : MetaM AssertAfterResult :=
-  -- mvarId.withContext do
-  --   let localDecl ← fvarId.getDecl
-  --   let typeNewPr ← mkIdMp eqProof (mkFVar fvarId)
-  --   let (_, localDecl') ← findMaxFVar typeNew |>.run localDecl
-  --   let result ← mvarId.assertAfter localDecl'.fvarId localDecl.userName typeNew typeNewPr
-  --   (do let mvarIdNew ← result.mvarId.clear fvarId
-  --       pure { result with mvarId := mvarIdNew })
-  --   <|> pure result
-  sorry
-
-def replaceLocalDeclObj (mvarId : MVarId) (fvarId : FVarId) (typeNew : Expr) (eqProof : Expr)
-                        : MetaM AssertAfterResult :=
-  replaceLocalDeclObjCore mvarId fvarId typeNew eqProof
+  return e.liftWith u
 
 /-- Given `h : ^(a =ₒ b)`, returns a proof of `b =ₒ a`. -/
 def mkIdSymm (h : Expr) : MetaM Expr := do
   if h.isAppOf ``Id.refl then
     return h
   else
-    let hType ← whnfD (← inferType h)
-    match ← hType.id? with
+    let hType ← inferType h
+    let hTypeₒ ← hType.objType!
+    match ← hTypeₒ.id? with
       | some (u, α, a, b) =>
-        return mkApp4 (mkConst ``Id.symm [u]) α a b h
+        return mkApp4 (.const ``Id.symm [u]) α a b h
       | none =>
         throwError "AppBuilder for '{``Id.symm}, object equality proof expected{indentExpr h}\nhas type{indentExpr hType}"
 
+/-- Returns `a =ₒ b`. -/
 def mkId (u : Level) (α a b : Expr) : MetaM Expr := do
-  return mkApp3 (mkConst ``Id [u]) α a b
+  return mkApp3 (.const ``Id [u]) α a b
 
 /-- Returns a proof of `a =ₒ a` if `a` is an object-level term. -/
 def mkIdRefl (a : Expr) : MetaM Expr := do
   let (u, aObjType) ← inferObjType a
-  return mkApp2 (mkConst ``Id.refl [u]) aObjType a
+  let result := mkApp2 (.const ``Id.refl [u]) aObjType a
+  return result
 
 def mkIdSubst (motive h idh : Expr) : MetaM Expr := do
   if (← whnfD idh).isAppOf ``Id.refl then
     return h
-  
   let (_, idhObjType) ← inferObjType idh
   match ← idhObjType.id? with
   | none => throwError "AppBuilder for '{``Id.subst}, object equality proof expected{indentExpr idh}\nhas type{indentExpr idhObjType}"
@@ -181,17 +175,22 @@ def mkIdSubst (motive h idh : Expr) : MetaM Expr := do
     let motiveType ← whnfD (← inferType motive)
     match motiveType with
     | .forallE _ _ motiveTargetType _ =>
-      let some (u₂, _) ← motiveTargetType.lift?
-        | throwError "Motive target type{indentExpr motiveTargetType}\nis not an object-level type"
-      return mkAppN (mkConst ``Id.subst [u₁, u₂]) #[α, motive, lhs, rhs, idh, h]
+      let some (_, U) ← motiveTargetType.lift?
+        | throwError "Motive target type{indentExpr motiveTargetType}\nis not a object-level universe type"
+      let u₂ ← mkFreshLevelMVar
+      let pattern := .const ``U [u₂]
+      if !(← isDefEq U pattern) then
+        throwError "Motive target type{indentExpr motiveTargetType}\nis not a object-level universe type"
+      return mkAppN (.const ``Id.subst [u₁, u₂]) #[α, motive, lhs, rhs, idh, h]
     | _ => throwError "AppBuilder for '{``Id.subst}, invalid motive{indentExpr motive}"
-
+    
+---  Object-level rewrite: rewriteₒ
 def rewriteObj (mvarId : MVarId) (e : Expr) (heq : Expr) (symm : Bool := false)
                (occs : Occurrences := .all) : MetaM RewriteResult :=
   mvarId.withContext do
     mvarId.checkNotAssigned `rewriteₒ
     let heqType ← instantiateMVars (← inferType heq)
-    let heqObjType ← heqType.objType
+    let heqObjType ← heqType.objType!
     let (newMVars, binderInfos, heqType) ← forallMetaTelescopeReducing heqType
     let heq := mkAppN heq newMVars
     match ← heqObjType.id? with
@@ -209,19 +208,16 @@ def rewriteObj (mvarId : MVarId) (e : Expr) (heq : Expr) (symm : Bool := false)
       if lhs.getAppFn.isMVar then
         throwTacticEx `rewriteₒ mvarId m!"pattern is a metavariable{indentExpr lhs}\nfrom equation{indentExpr heqType}"
       let e ← instantiateMVars e
-      let eAbst ← kabstract e lhs occs
-      unless eAbst.hasLooseBVars do
-        throwTacticEx `rewriteₒ mvarId m!"did not find instance of the pattern in the target expresion{indentExpr lhs}"
-      let eNew := eAbst.instantiate1 rhs
-      let eNew ← instantiateMVars eNew
       let some (e_level, e_obj) ← e.lift?
-        | throwTacticEx `rewriteₒ mvarId m!"the goal is not an object-level type{indentExpr e}"
-      let some e_abst_obj := eAbst.objType?
-        | throwTacticEx `rewriteₒ mvarId m!"the inferred context is not an object-level type"
-      let e_objeq_eabst ← mkId (.succ e_level) (.const ``U [e_level]) e_obj e_abst_obj
+        | throwTacticEx `rewriteₒ mvarId m!"the goal is not an object-level type"
+      let e_abstₒ ← kabstract e_obj lhs occs
+      unless e_abstₒ.hasLooseBVars do
+        throwTacticEx `rewriteₒ mvarId m!"did not find instance of the pattern in the target expresion{indentExpr lhs}"
+      let eNewₒ := e_abstₒ.instantiate1 rhs
+      let eNewₒ ← instantiateMVars eNewₒ
+      let e_objeq_eabst ← mkId (.succ e_level) (.const ``U [e_level]) e_obj e_abstₒ
       let liftedα ← α.lift
       let motive := Expr.lam `_a liftedα e_objeq_eabst BinderInfo.default
-      Lean.Meta.check motive
       unless ← isTypeCorrect motive do
         throwTacticEx `rewriteₒ mvarId "motive is not type correct..."
       let eqRefl ← mkIdRefl e_obj
@@ -231,23 +227,48 @@ def rewriteObj (mvarId : MVarId) (e : Expr) (heq : Expr) (symm : Bool := false)
       let otherMVarIds ← getMVarsNoDelayed eqPrf
       let otherMVarIds := otherMVarIds.filter (!newMVarIds.contains ·)
       let newMVarIds := newMVarIds ++ otherMVarIds
-      pure { eNew := eNew, eqProof := eqPrf, mvarIds := newMVarIds.toList }
+      pure { eNew := ← eNewₒ.lift, eqProof := eqPrf, mvarIds := newMVarIds.toList }
 
 def mkExpectedObjTypeHint (e : Expr) (expectedObjType : Expr) : MetaM Expr := do
   let u ← getObjLevel expectedObjType
-  return mkAppN (.const ``Arrow.id [u]) #[expectedObjType, e]
+  return mkAppN (.const ``id [.succ u]) #[expectedObjType.liftWith u, e]
+
+def replaceLocalDeclObj (mvarId : MVarId) (fvarId : FVarId) (typeNew : Expr)
+                        (eqProof : Expr) : MetaM AssertAfterResult :=
+  mvarId.withContext do
+    let localDecl ← fvarId.getDecl
+    let target ← fvarId.getType
+    let some (u, targetₒ) ← target.lift?
+      | throwTacticEx `rewriteₒ mvarId m!"target {indentExpr target}\nis not an object-level type"
+    let targetNewₒ ← typeNew.objType!
+    let typeNewPr := mkAppN (.const ``Id.mp [u]) #[targetₒ, targetNewₒ, eqProof, .fvar fvarId]
+    let (_, localDecl') ← findMaxFVar typeNew |>.run localDecl
+    let result ← mvarId.assertAfter localDecl'.fvarId localDecl.userName typeNew typeNewPr
+    (do let mvarIdNew ← result.mvarId.clear fvarId
+        pure { result with mvarId := mvarIdNew })
+    <|> pure result
+where
+  findMaxFVar (e : Expr) : StateRefT LocalDecl MetaM Unit :=
+    e.forEach' fun e => do
+      if e.isFVar then
+        let localDecl' ← e.fvarId!.getDecl
+        modify fun localDecl => if localDecl'.index > localDecl.index then localDecl' else localDecl
+        return false
+      else
+        return e.hasFVar
 
 def replaceTargetId (mvarId : MVarId) (targetNew : Expr) (eqProof : Expr) : MetaM MVarId :=
   mvarId.withContext do
     mvarId.checkNotAssigned `replaceTarget
     let tag ← mvarId.getTag
-    let mvarNew ← Lean.Meta.mkFreshExprSyntheticOpaqueMVar targetNew tag
+    let mvarNew ← mkFreshExprSyntheticOpaqueMVar targetNew tag
     let target ← mvarId.getType
-    let some (u, targetObjType) ← target.lift?
+    let some (u, targetₒ) ← target.lift?
       | throwTacticEx `rewriteₒ mvarId m!"target {indentExpr target}\nis not an object-level type"
-    let eq ← mkId u targetObjType target targetNew
+    let targetNewₒ ← targetNew.objType!
+    let eq ← mkId (.succ u) (.const ``U [u]) targetₒ targetNewₒ
     let newProof ← mkExpectedObjTypeHint eqProof eq
-    let val := mkAppN (Lean.mkConst ``Id.mpr [u]) #[target, targetNew, newProof, mvarNew]
+    let val := mkAppN (.const ``Id.mpr [u]) #[targetₒ, targetNewₒ, newProof, mvarNew]
     mvarId.assign val
     return mvarNew.mvarId!
 
@@ -259,13 +280,12 @@ def rewriteTarget (stx : Syntax) (symm : Bool) : TacticM Unit := do
     replaceMainGoal (mvarId' :: r.mvarIds)
 
 def rewriteLocalDecl (stx : Syntax) (symm : Bool) (fvarId : FVarId) : TacticM Unit := do
-  -- withSynthesize <| withMainContext do
-  --   let e ← elabTerm stx none true
-  --   let localDecl ← fvarId.getDecl
-  --   let rwResult ← rewriteObj (← getMainGoal) localDecl.type e symm
-  --   let replaceResult ← replaceLocalDeclObj (← getMainGoal) fvarId rwResult.eNew rwResult.eqProof
-  --   replaceMainGoal (replaceResult.mvarId :: rwResult.mvarIds)
-  pure ()
+  withSynthesize <| withMainContext do
+    let e ← elabTerm stx none true
+    let localDecl ← fvarId.getDecl
+    let rwResult ← rewriteObj (← getMainGoal) localDecl.type e symm
+    let replaceResult ← replaceLocalDeclObj (← getMainGoal) fvarId rwResult.eNew rwResult.eqProof
+    replaceMainGoal (replaceResult.mvarId :: rwResult.mvarIds)
 
 syntax (name := rewriteSeqObj) "rewriteₒ" rwRuleSeq (location)? : tactic
 
@@ -278,26 +298,97 @@ def rewriteSeqObjImpl : Tactic := fun stx => do
       (rewriteTarget term symm)
       (throwTacticEx `rewriteₒ · "did not find instance of the pattern in the current goal")
 
+namespace PathInduction
+  syntax (name := path_induction_obj) "path_inductionₒ " term (" with refl " term)? : tactic
 
-
-syntax (name := checkObj) "checkₒ" term : tactic
-
-@[tactic checkObj]
-def checkImpl : Tactic := fun stx => do
-  let e ← elabTerm stx[1] none true
-  let eType ← instantiateMVars (← inferType e)
-  match eType.objType? with
-  | none =>
+  def path_induction (path : FVarId) (name : Name) : TacticM Unit := do
     let mvarId ← getMainGoal
-    throwTacticEx `checkₒ mvarId "This term is not an object-level term"
-  | some t =>
-    Lean.logInfo s!"Term has object-level type {t}."
-    
--- set_option pp.universes true in
--- set_option trace.Meta.isDefEq true in
-example {α β : U.{0}} (h : β =ₒ α) (x : α) : β := by
+    mvarId.withContext do
+      let id_type ← path.getType
+      let path_expr ← id_type.objType!
+      let some (u, α, x, y) ← path_expr.id?
+        | throwTacticEx `path_inductionₒ mvarId
+                        m!"the variable {Expr.fvar path} has type{indentExpr id_type}\nwhile\n  ^(? =ₒ ?)\nwas expected"
+      let .fvar x_var ← instantiateMVars x
+        | throwTacticEx `path_inductionₒ mvarId m!"variable expected to induct on, got{indentExpr x}"
+      let .fvar y_var ← instantiateMVars y
+        | throwTacticEx `path_inductionₒ mvarId m!"variable expected to induct on, got{indentExpr y}"
+      -- we revert here, and intro later, because there might be other local hypothesis which
+      -- depend on `x_var`, `y_var` and `path`, which need to be reverted but not introed.
+      let (_, newGoal) ← mvarId.revert #[x_var, y_var, path] (preserveOrder := true)
+      newGoal.withContext do
+        let (motive, goal_level, newGoal) ← forallBoundedTelescope (← newGoal.getType) (some 3) fun args e => do
+          -- turn goals of the form (x : ^α) → ^β into ^((x : α) →ₒ β)
+          let (e, goal) ← forallTelescopeReducing e fun args e => do
+            let mut result := e
+            let mut goal := newGoal
+            for arg in args.reverse do
+              -- result =?= ^β
+              -- arg : ^α
+              -- goal : (arg : ^α) → result
+              let (u₂, β) ← result.lift!
+              let body ← mkLambdaFVars #[arg] β
+              let (u₁, α) ← inferObjType arg
+              result ← mkAppN (.const ``Pi [u₁, u₂]) #[α, body] |>.lift
+              -- goal' : ^((arg : α) →ₒ β)
+              let goal' ← mkFreshExprSyntheticOpaqueMVar result
+              goal.assign (mkAppN (.const ``Pi.app [u₁, u₂]) #[α, body, goal'])
+              goal := goal'.mvarId!
+            pure (result, goal)
+          let some (goal_level, motiveBody) ← e.lift?
+            | throwTacticEx `path_inductionₒ newGoal m!"the goal{indentExpr e}\nis not an object-level type"
+          return (← mkLambdaFVars args motiveBody, goal_level, goal)
+        let (goal, switcharoo) ← withLocalDecl name .default (← α.lift) fun newx => do
+          let motiveBody ←
+            whnfI (mkAppN motive #[newx, newx, mkApp2 (.const ``Id.refl [u]) α newx])
+          let liftedMotiveBody := motiveBody.liftWith goal_level
+          let body ← mkFreshExprSyntheticOpaqueMVar liftedMotiveBody
+          return (body, ← mkLambdaFVars #[newx] body)
+        let elimProof := mkAppN (.const ``Id.elim [u, goal_level]) #[α, motive, switcharoo]
+        replaceMainGoal [goal.mvarId!]
+        newGoal.assign elimProof
+
+  @[tactic path_induction_obj]
+  def path_induction_obj_impl : Tactic
+    | `(tactic| path_inductionₒ $p with refl $x) => do
+      let .ident _ _ name _ := x.raw
+        | throwTacticEx `path_inductionₒ (← getMainGoal) m!"expected variable, got {x}"
+      path_induction (← getFVarId p.raw) name
+    | `(tactic| path_inductionₒ $p) => do
+      path_induction (← getFVarId p.raw) `x
+    | _ => throwUnsupportedSyntax
+end PathInduction
+
+macro "rflₒ" : tactic => `(tactic| apply Id.refl)
+
+macro "rwₒ" s:rwRuleSeq l:(location)? : tactic =>
+  `(tactic| (rewriteₒ $s $(l)?; try (with_reducible rflₒ)))
+
+example {α β : U} (h : β =ₒ α) (x : α) : β := by
   rewriteₒ [h]
   assumption
-  -- exact x
+
+example (x y z : Natₒ) (h₁ : x =ₒ y) (h₂ : y =ₒ z) : x =ₒ z := by
+  rewriteₒ [h₁]
+  assumption
+
+example (x y z : Natₒ) (h₁ : x =ₒ y) (h₂ : y =ₒ z) : x =ₒ z := by
+  rewriteₒ [h₂] at h₁
+  assumption
+
+example (x y z : Natₒ) (h₁ : x =ₒ y) (h₂ : y =ₒ z) : x =ₒ z := by
+  rewriteₒ [h₁, h₂]
+  rflₒ
+
+example (x y z : Natₒ) (h₁ : x =ₒ y) (h₂ : y =ₒ z) : x =ₒ z := by
+  rwₒ [h₁, h₂]
+
+example (x y : Natₒ) (p : x =ₒ y) : y =ₒ x := by
+  path_inductionₒ p
+  rflₒ
+
+example {α β : U} (h : α =ₒ β) (x : α) : β := by
+  rewriteₒ [← h]
+  assumption
 
 end Hott.Tactic
